checkpoint

examples/algorithms/qsort_arr.fst
@@ -6,6 +6,12 @@ open ST
 open SeqProperties
 open SeqPermutation
 
+(* (\* Defining a new predicate symbol *\) *)
+(* type total_order (a:Type) (f: (a -> a -> Tot bool)) = *)
+(*     (forall a. f a a)                                           (\* reflexivity   *\) *)
+(*     /\ (forall a1 a2. (f a1 a2 /\ a1<>a2)  <==> not (f a2 a1))  (\* anti-symmetry *\) *)
+(*     /\ (forall a1 a2 a3. f a1 a2 /\ f a2 a3 ==> f a1 a3)        (\* transitivity  *\) *)
+
 let splice (a:Type) (s1:seq a) (i:nat) (s2:seq a{s1.length=s2.length})  (j:nat{i <= j /\ j <= s2.length})
     = Seq.append (slice s1 0 i) (Seq.append (slice s2 i j) (slice s1 j s1.length))
 
@@ -22,6 +28,7 @@ assume val partition: a:Type -> f:(a -> a -> Tot bool){total_order a f}
            /\ (back < i  ==> f (index (sel h x) pivot) (index (sel h x) i))))))
   (ensures (fun h0 i h1 -> 
     len <= length (sel h0 x)
+    /\ contains h1 x
     /\ start <= i 
     /\ i < len
     /\ (length (sel h1 x) = length (sel h0 x))
@@ -41,71 +48,36 @@ val sort: a:Type -> f:(a -> a -> Tot bool){total_order a f} -> i:nat -> j:nat{i 
           -> x:array a -> ST unit 
   (requires (fun h -> contains h x /\ j <= length (sel h x)))
   (ensures (fun h0 u h1 -> (j <= length (sel h0 x)
+                            /\ contains h1 x
                             /\ (length (sel h0 x) = length (sel h1 x))
                             /\ sorted f (slice (sel h1 x) i j)
                             /\ (sel h1 x = splice (sel h0 x) i (sel h1 x) j)
                             /\ permutation a (slice (sel h0 x) i j) (slice (sel h1 x) i j))))
   (modifies (a_ref x))
 let rec sort f i j x = 
+  let h0 = ST.get () in
   if i=j 
-  then admit()
-  else begin
-    (* let h0 = ST.get () in  *)
+  then cut (Eq (sel h0 x) (splice (sel h0 x) i (sel h0 x) j))
+  else 
     let pivot = partition f i j i (j - 1) x in
-    (* let h1 = ST.get () in  *)
+    let h1 = ST.get () in
     sort f i pivot x;
     (* let h2 = ST.get () in  *)
     sort f (pivot + 1) j x;
+    admit ()
+
     (* let h3 = ST.get () in  *)
     (* assert (sel h1 x = splice (sel h0 x) i (sel h1 x) j); *)
     (* assert (sorted f (slice (sel h2 x) i pivot)); *)
     (* assert (sorted f (slice (sel h3 x) (pivot + 1) j)); *)
-    (* let l = slice (sel h3 x) i pivot in *)
-    (* let pv = index (sel h1 x) pivot in *)
-    (* let h = slice (sel h3 x) (pivot + 1) j in *)
-    (* let hi = slice (sel h1 x) pivot j in *)
-    (* assert (Eq (slice (sel h3 x) i j)  *)
-    (*           (append (slice (sel h3 x) i pivot)  *)
-    (*                   (cons (index (sel h1 x) pivot) *)
-    (*                         (slice (sel h3 x) (pivot + 1) j)))); *)
-    admit ()
-    (* sorted_concat_lemma f l pv h; *)
-    (* assert (sorted f (append l (cons pv h))); *)
-    (* lemma_append_count l (cons pv h); *)
-    (* cons_perm h hi; *)
-    (* admitP (b2t (sel h3 x = splice (sel h0 x) i (sel h3 x) j)) *)
-  end
-
-(* let rec sort f i j x =  *)
-(*   let h0 = ST.get () in  *)
-(*   if i=j  *)
-(*   then cut (Eq (sel h0 x) (splice (sel h0 x) i (sel h0 x) j)) *)
-(*   else begin *)
-(*     let pivot = partition f i j i (j - 1) x in *)
-(*     let h1 = ST.get () in  *)
-(*     sort f i pivot x; *)
-(*     let h2 = ST.get () in  *)
-(*     sort f (pivot + 1) j x; *)
-(*     let h3 = ST.get () in  *)
-(*     assert (sel h1 x = splice (sel h0 x) i (sel h1 x) j); *)
-(*     assert (sorted f (slice (sel h2 x) i pivot)); *)
-(*     assert (sorted f (slice (sel h3 x) (pivot + 1) j)); *)
-(*     let l = slice (sel h3 x) i j in *)
-(*     let pv = index (sel h1 x) pivot in *)
-(*     let h = slice (sel h3 x) (pivot + 1) j in *)
-(*     let hi = slice (sel h1 x) pivot j in *)
-(*     assert (Eq (slice (sel h3 x) i j) (append l (cons pv h))); *)
-(*     admit () *)
-(*     (\* sorted_concat_lemma f l pv h; *\) *)
-(*     (\* assert (sorted f (append l (cons pv h))); *\) *)
-(*     (\* lemma_append_count l (cons pv h); *\) *)
-(*     (\* cons_perm h hi; *\) *)
-(*     (\* admitP (b2t (sel h3 x = splice (sel h0 x) i (sel h3 x) j)) *\) *)
-(*   end *)
-
+    (* assert (Eq (slice (sel h3 x) i j) *)
+    (*            (append (slice (sel h2 x) i pivot) *)
+    (*                    (cons (index (sel h1 x) pivot) *)
+    (*                          (slice (sel h3 x) (pivot + 1) j)))); *)
+    (* admit () *)
        
 
-(* (\* val qsort: a:Type -> f:(a -> a -> Tot bool){total_order a f} -> x:array a -> ST unit  *\) *)
-(* (\*   (requires (fun h -> contains h x)) *\) *)
-(* (\*   (ensures (fun h0 u h1 -> sorted f (sel h1 x) /\ permutation a (sel h0 x) (sel h1 x))) *\) *)
-(* (\*   (modifies (a_ref x)) *\) *)
+(* val qsort: a:Type -> f:(a -> a -> Tot bool){total_order a f} -> x:array a -> ST unit  *)
+(*   (requires (fun h -> contains h x)) *)
+(*   (ensures (fun h0 u h1 -> sorted f (sel h1 x) /\ permutation a (sel h0 x) (sel h1 x))) *)
+(*   (modifies (a_ref x)) *)
